created a version of `traverse` on expr that produces a proof that the size does not increase
It is used in `is_free e` which checks if local variable `n+1` is free in `e` and adapts the type of `e` if not.

ski.lean
@@ -14,6 +14,9 @@ if h' : v < n
 then f (var.bound _ ⟨v,h'⟩)
 else x
 
+def var.split {α : Type u} {n : ℕ} : var α (n+1) → option (var α n) :=
+var.rec' none some
+
 def bound {α : Type u} {n : ℕ} : var α (n+1) :=
 var.bound _ ⟨n,nat.lt_succ_self n⟩
 
@@ -23,13 +26,13 @@ def bump {α : Type u} {n : ℕ} : var α n → var α (n+1)
 
 open has_map
 
-def dumped {α α' : Type u} {n n' : ℕ} {f : Type u → Type v} [applicative f]
+def dumping {α α' : Type u} {n n' : ℕ} {f : Type u → Type v} [applicative f]
   (F : var α n → f (var α' n'))
 : var α (n+1) → f (var α' (n'+1)) :=
 var.rec' (pure bound) (map bump ∘ F)
 
 inductive expr (t : Type u) (α : Type u) : ℕ → Type u
-  | var {} (n : ℕ) : var α n → expr n
+  | var {n : ℕ} : var α n → expr n
   | app {n : ℕ} : expr n → expr n → expr n
   | abstr (n : ℕ) : t → expr (n+1) → expr n
   | skip {n : ℕ} : expr n → expr (n+1)
@@ -55,7 +58,7 @@ def instantiate {α γ : Type u} {n : ℕ}
   (v : α)
   (e : expr γ α (n+1))
 : expr γ α n :=
-bind e (var.rec' (expr.var _ $ var.free _ v) (expr.var n))
+bind e (var.rec' (expr.var _ $ var.free _ v) (@expr.var _ _ n))
 
 def abstract {γ α : Type u} {n : ℕ}
   (p : α) [decidable_eq α]
@@ -68,15 +71,97 @@ match v with
  | (var.bound ._ v) := bump $ var.bound α v
 end
 
+def size {t α : Type u} : ∀ {n : ℕ}, expr t α n → ℕ
+ | n (expr.var ._ _)  := 0
+ | n (expr.app e₀ e₁) := 1 + size e₀ + size e₁
+ | n (expr.abstr ._ _ e) := 1 + size e
+ | ._ (@expr.skip ._ ._ n e)   := 1 + size e
+
 def traverse {f : Type u → Type v} [applicative f] {t α α' : Type u}
 : ∀ {n n'},
   (var α n → f (var α' n')) →
   expr t α n → f (expr t α' n')
 | n n' f (expr.var ._ v) := expr.var _ <$> f v
 | n n' f (expr.app e₀ e₁) := expr.app <$> traverse f e₀ <*> traverse f e₁
-| n n' f (expr.abstr ._ t e) := expr.abstr _ t <$> traverse (dumped f) e
-| (n+1) n' f (expr.skip e) := traverse (f ∘ bump) e
+| n n' f (expr.abstr ._ t e) := expr.abstr _ t <$> traverse (dumping f) e
+| (nat.succ n) n' f (expr.skip e) := traverse (f ∘ bump) e
 
+inductive expr.rel {t α α' : Type u} (P : ∀ {n n' : ℕ}, var α n → var α' n' → Prop)
+: ∀ {n n'}, expr t α n → expr t α' n' → Prop
+  | basis {i j} {v : var α i} {v' : var α' j} :
+         P v v' → expr.rel (expr.var _ v) (expr.var _ v')
+  | app {i j} {e₀ e₁ : expr t α i} {e₀' e₁' : expr t α' j} :
+         expr.rel e₀ e₀' →
+         expr.rel e₁ e₁' →
+         expr.rel (expr.app e₀ e₁) (expr.app e₀' e₁')
+  | abstr {i j} {x y : t} {e : expr t α $ i+1} {e' : expr t α' $ j+1} :
+         expr.rel e e' →
+         expr.rel (expr.abstr _ x e) (expr.abstr _ y e')
+  | skip {i j} {e : expr t α i} {e' : expr t α' j} :
+         expr.rel e e' →
+         expr.rel (expr.skip e) e'
+  | skip' {i j} {e : expr t α i} {e' : expr t α' j} :
+         expr.rel e e' →
+         expr.rel e (expr.skip e')
+
+def dec_t {t α : Type u} {n : ℕ} (α' : Type u) (n' : ℕ) (x : expr t α n) :=
+{ y : expr t α' n' // size y ≤ size x }
+
+def expr_wf {t α : Type u} {n : ℕ}
+: has_well_founded (expr t α n) :=
+⟨ measure size, measure_wf size ⟩
+
+def mk_var {t α α' : Type u} {n n' : ℕ}
+  {v  : var α n}
+  (v' : var α' n')
+: dec_t α' n' (expr.var t v) :=
+⟨ expr.var _ v', by simp [size] ⟩
+
+def mk_app  {t α α' : Type u} {n n' : ℕ}
+  {e₀ e₁ : expr t α n}
+  (e₀' : dec_t α' n' e₀)
+  (e₁' : dec_t α' n' e₁)
+: dec_t α' n' (expr.app e₀ e₁) :=
+have h : size (expr.app (e₀'.val) (e₁'.val)) ≤ size (expr.app e₀ e₁),
+  begin
+    simp [size],
+    apply add_le_add_left,
+    apply add_le_add e₀'.property e₁'.property
+  end,
+⟨ expr.app e₀'.val e₁'.val, h ⟩
+
+def mk_abstr  {t α α' : Type u} {n n' : ℕ}
+  {i : t} {e  : expr t α (n + 1)}
+  (e' : dec_t α' (n' + 1) e)
+: dec_t α' n' (expr.abstr n i e) :=
+have size (expr.abstr n' i (e'.val)) ≤ size (expr.abstr n i e),
+  by { simp [size], apply add_le_add_left, apply e'.property },
+⟨ expr.abstr _ i e'.val , this ⟩
+
+def mk_skip  {t α α' : Type u} {n n' : ℕ}
+  {e  : expr t α n}
+  (e' : dec_t α' n' e)
+: dec_t α' n' (expr.skip e) :=
+have size (e'.val) ≤ size (expr.skip e),
+ by { simp [size],
+      transitivity size e,
+      { apply e'.property },
+      { apply nat.le_add_left } },
+⟨ e'.val, this ⟩
+
+def traverse' {f : Type u → Type v} [applicative f] {t α α' : Type u}
+: ∀ {n n'},
+  (var α n → f (var α' n')) →
+  ∀ e : expr t α n, f (dec_t α' n' e)
+| n n' f (expr.var ._ v) :=
+  mk_var <$> f v
+| n n' f (expr.app e₀ e₁) :=
+  mk_app <$> traverse' f e₀
+         <*> traverse' f e₁
+| n n' f (expr.abstr ._ i e) :=
+  mk_abstr <$> traverse' (dumping f) e
+| (n+1) n' f (expr.skip e) :=
+  mk_skip <$> traverse' (f ∘ bump) e
 
 inductive ski (α : Type u) : Type u
   | S {} : ski
@@ -85,43 +170,50 @@ inductive ski (α : Type u) : Type u
   | var {} : α → ski
 
 def K {t α : Type u} {n : ℕ} : expr t (ski α) n :=
-expr.var n (var.free n ski.K)
-
+expr.var _ (var.free n ski.K)
 
 def is_free {t α : Type u} {n : ℕ} (e : expr t α (n+1))
-: option (expr t α n) :=
-traverse (var.rec' none some) e
+: option (dec_t α n e) :=
+traverse' (var.rec' none some) e
 
-section well_founded_tactics
 
-open tactic well_founded_tactics
 
-meta def my_wf_tac : well_founded_tactics :=
-{ rel_tac := λ _ _, trace_state >> apply_instance
-, dec_tac := do
-    clear_internals,
-    unfold_wf_rel,
-    process_lex (unfold_sizeof >> assumption <|> (cancel_nat_add_lt >> trivial_nat_lt))
-}
 
 end well_founded_tactics
+
+lemma nat.lt_add_of_zero_lt_right (a b : nat) (h : 0 < a) : b < a + b :=
+suffices 0 + b < a + b, by {simp at this, assumption},
+by {apply nat.add_lt_add_right, assumption}
+
+lemma nat.foo_left {a b k : ℕ}
+  (h  : 0 < k)
+  (h' : a ≤ b)
+: a < k + b := sorry
+
+lemma nat.foo_right {a b k : ℕ}
+  (h  : 0 < k)
+  (h' : a ≤ b)
+: a < b + k := sorry
+
+local attribute [instance] expr_wf
 
 def to_ski {α : Type u}
 : ∀ {n}, expr (ulift unit) α n → expr (ulift empty) (ski α) n
  | n (expr.var ._ v) := expr.var _ $ var.rec_on v (var.free _ ∘ ski.var) (var.bound _)
  | n (expr.app e₀ e₁) :=
-   have sizeof_measure ℕ n n, from sorry,
+   have size e₀ < 1 + size e₀ + size e₁,
+     by { apply nat.lt_add_right, apply nat.foo_left, apply zero_lt_one, refl },
+   have size e₁ < 1 + size e₀ + size e₁,
+     by { apply nat.foo_left, apply nat.zero_lt_one_add, refl },
    expr.app (to_ski e₀) (to_ski e₁)
  | n (expr.abstr ._ t e) :=
-   let x := is_free e in
-   have h : x = is_free e, from rfl,
-   match x, h with
-    | (some e'), h :=
-      have h : sizeof e' < n + (1 + (sizeof t + sizeof e)), from sorry,
-      expr.app K (to_ski e')
-    | none, _ := sorry
+   match is_free e with
+    | (some e') :=
+      have h : size e'.val < 1 + size e,
+        by { apply nat.foo_left, apply zero_lt_one, apply e'.property },
+      expr.app K (to_ski e'.val)
+    | none := sorry
    end
- | (n+1) (expr.skip e) := sorry
-using_well_founded my_wf_tac
+ | (n+1) (expr.skip e) := expr.skip $ to_ski e
 
 end ski
